% Created 2019-05-25 Sat 14:02
% Intended LaTeX compiler: pdflatex
\documentclass[11pt]{article}
\usepackage[utf8]{inputenc}
\usepackage[T1]{fontenc}
\usepackage{graphicx}
\usepackage{grffile}
\usepackage{longtable}
\usepackage{wrapfig}
\usepackage{rotating}
\usepackage[normalem]{ulem}
\usepackage{amsmath}
\usepackage{textcomp}
\usepackage{amssymb}
\usepackage{capt-of}
\usepackage{hyperref}
\usepackage{amsmath}
\usepackage{mathtools}
\usepackage[english, russian]{babel}
\author{Sergey Makarov}
\date{\today}
\title{}
\hypersetup{
 pdfauthor={Sergey Makarov},
 pdftitle={},
 pdfkeywords={},
 pdfsubject={},
 pdfcreator={Emacs 26.2 (Org mode 9.1.9)}, 
 pdflang={English}}
\begin{document}

\section{Задача 4(а)}
\label{sec:org6bda04a}
Вычислить интеграл:
$$\int_1^3\sqrt\frac{x - 1}{3 - x}\frac{dx}{(x + 2)^2}$$

\begin{multline*}
\int_1^3\sqrt\frac{x - 1}{3 - x}\frac{dx}{(x + 2)^2} = \int_1^3(x - 1)^{\frac12}(3 - x)^{-\frac12}(x + 2)^{-2}dx
=\bigg|_{t = \frac{x - 1}2}\int_0^1{2t}^\frac12(2 - 2t)^{-\frac12}(3 + 2t)^{-2}dt = \\
= \frac14\int_0^1t^{\frac12}(1 - t)^{-\frac12}\left(\frac32 + t\right)^{-2}dt
\end{multline*}
Положим \(t = \frac{x - 1}{3 - x} = -1 + \frac{2}{3 - x}\). Тогда:
$$3 - x = \frac2{t + 1} \Rightarrow x = 3 - \frac2{t + 1} = \frac{3t + 1}{t + 1}$$
$$dx = -2d{\frac1{t + 1}} = \frac{2dt}{(t + 1)^2}$$
$$\frac1{(x + 2)^2} = \frac1{\left(5 - \frac2{t + 1}\right)^2} = \frac{(t + 1)^2}{(5t + 3)^2}$$
\end{document}
